Major change to smtlink hint interface

books/projects/smtlink/trusted/trusted-cp.lisp
@@ -34,13 +34,10 @@
 
     (define SMT-trusted-cp-main ((cl pseudo-term-listp)
                                  (smtlink-hint)
-                                 (custom-p booleanp)
                                  state)
       :stobjs state
       :mode :program
-      (b* ((smt-cnf (if custom-p (custom-smt-cnf) (default-smt-cnf)))
-           (smtlink-hint (change-smtlink-hint smtlink-hint :smt-cnf smt-cnf))
-           ((mv res smt-precond uninterpreted-precond state)
+      (b* (((mv res smt-precond uninterpreted-precond state)
             (SMT-prove-stub (disjoin cl) smtlink-hint state))
            (subgoal-lst `(((hint-please
                             '(:in-theory (enable magic-fix
@@ -67,7 +64,7 @@
     :mode :program
     :stobjs state
     (prog2$ (cw "Using default SMT-trusted-cp...~%")
-            (SMT-trusted-cp-main cl smtlink-hint nil state)))
+            (SMT-trusted-cp-main cl smtlink-hint state)))
 
   (define SMT-trusted-cp-custom ((cl pseudo-term-listp)
                                  (smtlink-hint smtlink-hint-p)
@@ -75,7 +72,7 @@
     :mode :program
     :stobjs state
     (prog2$ (cw "Using custom SMT-trusted-cp...~%")
-            (SMT-trusted-cp-main cl smtlink-hint t state)))
+            (SMT-trusted-cp-main cl smtlink-hint state)))
 
   (define-trusted-clause-processor
     SMT-trusted-cp
