books/projects/smtlink/trusted/z3-py/recover-uninterpreted.lisp
@@ -10,11 +10,10 @@
 (include-book "std/util/define" :dir :system)
 (include-book "ordinals/lexicographic-ordering-without-arithmetic" :dir :system)
 (include-book "../../verified/hint-interface")
-(include-book "../../verified/pseudo-lambda-lemmas")
 
-(defsection SMT-recover-uninterpreted
-  :parents (z3-py)
-  :short "Recovering return types of uninterpreted functions"
+;; (defsection SMT-recover-uninterpreted
+;;   :parents (z3-py)
+;;   :short "Recovering return types of uninterpreted functions"
 
   (defprod fix-guard
     ((fixer symbolp)
@@ -45,14 +44,6 @@
           t))
       nil))
 
-  (define find-guard-for-fixing ((fn-call symbolp)
-                                 (fty-info fty-info-alist-p))
-    :returns (guard symbolp)
-    (b* (((mv & flex-guard) (fixing-of-flextype fn-call fty-info))
-         (base-guard (fixing-of-basetype fn-call *SMT-fixers*))
-         (guard (if (consp flex-guard) (car flex-guard) base-guard)))
-      guard))
-
   (defines recover-uninterpreted
     :well-founded-relation l<
     :flag-local nil
@@ -60,42 +51,42 @@
     :verify-guards nil
 
     (define recover-uninterpreted-list ((term-lst pseudo-term-listp)
-                                        (fn-alst func-alistp)
-                                        (fty-info fty-info-alist-p)
-                                        (fn-acc func-alistp)
+                                        (fn-lst smt-function-list-p)
+                                        (fixtypes smt-fixtype-list-p)
+                                        (fn-acc smt-function-list-p)
                                         (fix-alst fn-fix-alist-p))
       :returns (mv (new-term-lst pseudo-term-listp)
-                   (new-fn-acc func-alistp)
+                   (new-fn-acc smt-function-list-p)
                    (new-fix-alst fn-fix-alist-p))
       :measure (acl2-count (pseudo-term-list-fix term-lst))
       :hints (("Goal" :in-theory (enable pseudo-term-list-fix
                                          pseudo-term-fix)))
       (b* ((term-lst (pseudo-term-list-fix term-lst))
-           (fn-acc (func-alist-fix fn-acc))
+           (fn-acc (smt-function-list-fix fn-acc))
            (fix-alst (fn-fix-alist-fix fix-alst))
            ((unless (consp term-lst)) (mv term-lst fn-acc fix-alst))
            ((cons first rest) term-lst)
            ((mv first-term first-fn-acc first-fix-alst)
-            (recover-uninterpreted first fn-alst fty-info fn-acc fix-alst))
+            (recover-uninterpreted first fn-lst fixtypes fn-acc fix-alst))
            ((mv rest-term-lst rest-fn-acc rest-fix-alst)
-            (recover-uninterpreted-list rest fn-alst fty-info
+            (recover-uninterpreted-list rest fn-lst fixtypes
                                         first-fn-acc first-fix-alst)))
         (mv (cons first-term rest-term-lst)
             rest-fn-acc
             rest-fix-alst)))
 
     (define recover-uninterpreted ((term pseudo-termp)
-                                   (fn-alst func-alistp)
-                                   (fty-info fty-info-alist-p)
-                                   (fn-acc func-alistp)
+                                   (fn-lst smt-function-list-p)
+                                   (fixtypes smt-fixtype-list-p)
+                                   (fn-acc smt-function-list-p)
                                    (fix-alst fn-fix-alist-p))
       :returns (mv (new-term pseudo-termp)
-                   (new-fn-acc func-alistp)
+                   (new-fn-acc smt-function-list-p)
                    (new-fix-alst fn-fix-alist-p))
       :measure (acl2-count (pseudo-term-fix term))
       (b* ((term (pseudo-term-fix term))
-           (fn-alst (func-alist-fix fn-alst))
-           (fn-acc (func-alist-fix fn-acc))
+           (fn-lst (smt-function-list-fix fn-lst))
+           (fn-acc (smt-function-list-fix fn-acc))
            (fix-alst (fn-fix-alist-fix fix-alst))
            ;; If first term is a symbolp or is quoted, return the current facts
            ((if (or (acl2::variablep term) (acl2::fquotep term)))
@@ -117,14 +108,14 @@
            ;; If it is a fixing function, first check fix-alst to see if (caar
            ;; fn-actuals) exists and if it's fixer is the same fixer.
            ;; we find out what its type recognizer is and compare it with the
-           ;; fn-alst table. If they don't match, complain; otherwise build an
+           ;; fn-lst table. If they don't match, complain; otherwise build an
            ;; item for new-fn-acc and an item for new-fix-alst
            ;; If the function is not a fixing function, continue with the
            ;; arguments.
-           (guard (find-guard-for-fixing fn-call fty-info))
+           (guard (recognizer-of-fixer fn-call fixtypes))
            ((unless guard)
             (b* (((mv rest-term-lst rest-fn-acc rest-fix-alst)
-                  (recover-uninterpreted-list fn-actuals fn-alst fty-info fn-acc
+                  (recover-uninterpreted-list fn-actuals fn-lst fixtypes fn-acc
                                               fix-alst)))
               (mv (cons fn-call rest-term-lst)
                   rest-fn-acc
@@ -133,9 +124,9 @@
                          (null (cdr fn-actuals))
                          (consp (car fn-actuals))
                          (symbolp (caar fn-actuals))
-                         (assoc-equal (caar fn-actuals) fn-alst)))
+                         (is-function (caar fn-actuals) fn-lst)))
             (b* (((mv rest-term-lst rest-fn-acc rest-fix-alst)
-                  (recover-uninterpreted-list fn-actuals fn-alst fty-info fn-acc
+                  (recover-uninterpreted-list fn-actuals fn-lst fixtypes fn-acc
                                               fix-alst)))
               (mv (cons fn-call rest-term-lst)
                   rest-fn-acc
@@ -147,28 +138,29 @@
                         (caar fn-actuals) (fix-guard->fixer (cdr exist?)) fn-call)
                     (mv nil nil nil)))
            ((if exist?)
-            (recover-uninterpreted (car fn-actuals) fn-alst fty-info fn-acc
+            (recover-uninterpreted (car fn-actuals) fn-lst fixtypes fn-acc
                                    fix-alst))
-           (func (cdr (assoc-equal (caar fn-actuals) fn-alst)))
-           (returns (func->returns func))
+           (func (is-function (caar fn-actuals) fn-lst))
+           (returns (smt-function->returns func))
            ((unless (and (consp returns)
                          (null (cdr returns))))
             (prog2$ (er hard? 'recover-uninterpreted=>recover-uninterpreted
                         "Uninterpreted function returns wrong: ~q0" func)
                     (mv nil nil nil)))
            (typep (hint-pair->thm (decl->type (car returns))))
-           ((unless (ambiguous-equal guard typep))
+           ((unless (and (type-decl-p typep fixtypes)
+                         (ambiguous-equal guard (car typep))))
             (prog2$ (er hard? 'recover-uninterpreted=>recover-uninterpreted
                         "Guard for fixing function ~p0 is ~p1, but user defined
 function ~p2 returns ~p3~%" fn-call guard (caar fn-actuals) typep)
                     (mv nil nil nil)))
-           (new-fn-acc (acons (caar fn-actuals) func fn-acc))
+           (new-fn-acc (cons func fn-acc))
            (new-fix-alst (acons (caar fn-actuals)
                                 (make-fix-guard :fixer fn-call
                                                 :guard guard)
                                 fix-alst))
            ((mv rest-term rest-fn-acc rest-fix-alst)
-            (recover-uninterpreted (car fn-actuals) fn-alst fty-info new-fn-acc
+            (recover-uninterpreted (car fn-actuals) fn-lst fixtypes new-fn-acc
                                    new-fix-alst)))
         (mv rest-term rest-fn-acc rest-fix-alst)))
     )
@@ -202,17 +194,17 @@ function ~p2 returns ~p3~%" fn-call guard (caar fn-actuals) typep)
             (construct-uninterpreted-precond rest (cons fg.fixer acc) state))))
 
   (define recover-uninterpreted-top ((term pseudo-termp)
-                                     (fn-alst func-alistp)
-                                     (fty-info fty-info-alist-p)
+                                     (fn-lst smt-function-list-p)
+                                     (fixtypes smt-fixtype-list-p)
                                      state)
     ;; :returns (mv (new-term pseudo-termp)
-    ;;              (new-fn-alst func-alistp)
+    ;;              (new-fn-lst smt-function-list-p)
     ;;              (uninterpreted-precond pseudo-term-list-listp))
     :mode :program
-    (b* (((mv new-term new-fn-alst new-fix-alst)
-          (recover-uninterpreted term fn-alst fty-info nil nil))
+    (b* (((mv new-term new-fn-lst new-fix-alst)
+          (recover-uninterpreted term fn-lst fixtypes nil nil))
          (uninterpreted-precond
           (construct-uninterpreted-precond new-fix-alst nil state)))
-      (mv new-term new-fn-alst uninterpreted-precond)))
+      (mv new-term new-fn-lst uninterpreted-precond)))
 
-  )
+;;  )
