books/projects/smtlink/utils/basics.lisp
@@ -1,0 +1,138 @@
+;; Copyright (C) 2015, University of British Columbia
+;; Written by Yan Peng (June 25th 2019)
+;;
+;; License: A 3-clause BSD license.
+;; See the LICENSE file distributed with ACL2
+;;
+(in-package "SMT")
+(include-book "centaur/fty/top" :dir :system)
+(include-book "xdoc/top" :dir :system)
+(include-book "std/util/define" :dir :system)
+
+(include-book "pseudo-lambda-lemmas")
+
+(define pseudo-term-fix ((x pseudo-termp))
+  :returns (fixed pseudo-termp)
+  (mbe :logic (if (pseudo-termp x) x nil)
+       :exec x)
+  ///
+  (more-returns
+   (fixed (implies (pseudo-termp x) (equal fixed x))
+          :name equal-fixed-and-x-of-pseudo-termp)))
+
+(defthm pseudo-term-fix-idempotent-lemma
+  (equal (pseudo-term-fix (pseudo-term-fix x))
+         (pseudo-term-fix x))
+  :hints (("Goal" :in-theory (enable pseudo-term-fix))))
+
+(deffixtype pseudo-term
+  :fix pseudo-term-fix
+  :pred pseudo-termp
+  :equiv pseudo-term-equiv
+  :define t
+  :forward t
+  :topic pseudo-termp)
+
+(define pseudo-term-list-fix ((x pseudo-term-listp))
+  :returns (new-x pseudo-term-listp)
+  (mbe :logic (if (consp x)
+                  (cons (pseudo-term-fix (car x))
+                        (pseudo-term-list-fix (cdr x)))
+                nil)
+       :exec x)
+  ///
+  (more-returns
+   (new-x (<= (acl2-count new-x) (acl2-count x))
+          :name acl2-count-<=-pseudo-term-list-fix
+          :rule-classes :linear
+          :hints (("Goal" :in-theory (enable pseudo-term-fix))))
+   (new-x (implies (pseudo-term-listp x)
+                   (equal new-x x))
+          :name equal-pseudo-term-list-fix)
+   (new-x (implies (pseudo-term-listp x)
+                   (equal (len new-x) (len x)))
+          :name len-equal-pseudo-term-list-fix
+          :rule-classes :linear)))
+
+(defthm pseudo-term-list-fix-idempotent-lemma
+  (equal (pseudo-term-list-fix (pseudo-term-list-fix x))
+         (pseudo-term-list-fix x))
+  :hints (("Goal" :in-theory (enable pseudo-term-list-fix))))
+
+(deffixtype pseudo-term-list
+  :fix pseudo-term-list-fix
+  :pred pseudo-term-listp
+  :equiv pseudo-term-list-equiv
+  :define t)
+
+(defthmd pseudo-term-listp-of-cdr-pseudo-termp
+  (implies (and (pseudo-termp term)
+                (consp term)
+                (not (equal (car term) 'quote)))
+           (pseudo-term-listp (cdr term)))
+  :hints (("Goal" :in-theory (enable pseudo-termp))))
+
+(defthmd pseudo-termp-of-car-of-pseudo-term-listp
+  (implies (and (pseudo-term-listp term)
+                (consp term))
+           (pseudo-termp (car term))))
+
+(define pseudo-term-list-list-fix ((x pseudo-term-list-listp))
+  :returns (fixed pseudo-term-list-listp)
+  (mbe :logic (if (consp x)
+                  (cons (pseudo-term-list-fix (car x))
+                        (pseudo-term-list-list-fix (cdr x)))
+                nil)
+       :exec x))
+
+(defthm pseudo-term-list-list-fix-idempotent-lemma
+  (equal (pseudo-term-list-list-fix (pseudo-term-list-list-fix x))
+         (pseudo-term-list-list-fix x))
+  :hints (("Goal" :in-theory (enable pseudo-term-list-list-fix))))
+
+(deffixtype pseudo-term-list-list
+  :fix pseudo-term-list-list-fix
+  :pred pseudo-term-list-listp
+  :equiv pseudo-term-list-list-equiv
+  :define t
+  :forward t
+  :topic pseudo-term-list-listp)
+
+(defalist pseudo-term-alist
+  :key-type pseudo-term
+  :val-type pseudo-term
+  :pred pseudo-term-alistp
+  :true-listp t)
+
+(define true-list-fix ((lst true-listp))
+  :parents (SMT-hint-interface)
+  :short "Fixing function for true-listp."
+  :returns (fixed-lst true-listp)
+  (mbe :logic (if (consp lst)
+                  (cons (car lst)
+                        (true-list-fix (cdr lst)))
+                nil)
+       :exec lst))
+
+(defthm true-list-fix-idempotent-lemma
+  (equal (true-list-fix (true-list-fix x))
+         (true-list-fix x))
+  :hints (("Goal" :in-theory (enable true-list-fix))))
+
+(defthm true-list-fix-preserve-length
+  (equal (len (true-list-fix x))
+         (len x))
+  :hints (("Goal" :in-theory (enable true-list-fix))))
+
+(defthm true-list-fix-when-true-listp
+  (implies (true-listp x)
+           (equal (true-list-fix x) x))
+  :hints (("Goal" :in-theory (enable true-listp true-list-fix))))
+
+(deffixtype true-list
+  :fix true-list-fix
+  :pred true-listp
+  :equiv true-list-equiv
+  :define t
+  :forward t
+  :topic true-listp)
