books/projects/smtlink/verified/hint-interface.lisp
@@ -11,390 +11,273 @@
 (include-book "std/util/define" :dir :system)
 
 (include-book "../config")
-(include-book "fty")
+(include-book "../utils/basics")
 
 (defsection SMT-hint-interface
   :parents (verified)
   :short "Define default Smtlink hint interface"
 
-  ;; -------------------------------------------------------
-  ;;
-  ;; Define default Smtlink hint interface
-  ;;
-  ;;  One needs to attach to SMT-hint their own aggregate
-  ;;    to pass in a different hint.
-  ;;
-
-  (define pseudo-term-fix ((x pseudo-termp))
-    :returns (fixed pseudo-termp)
-    (mbe :logic (if (pseudo-termp x) x nil)
-         :exec x)
-    ///
-    (more-returns
-     (fixed (implies (pseudo-termp x) (equal fixed x))
-            :name equal-fixed-and-x-of-pseudo-termp)))
-
-  (defthm pseudo-term-fix-idempotent-lemma
-    (equal (pseudo-term-fix (pseudo-term-fix x))
-           (pseudo-term-fix x))
-    :hints (("Goal" :in-theory (enable pseudo-term-fix))))
-
-  (deffixtype pseudo-term
-    :fix pseudo-term-fix
-    :pred pseudo-termp
-    :equiv pseudo-term-equiv
-    :define t
-    :forward t
-    :topic pseudo-termp)
-
-  (define pseudo-term-list-fix ((x pseudo-term-listp))
-    :returns (new-x pseudo-term-listp)
-    (mbe :logic (if (consp x)
-                    (cons (pseudo-term-fix (car x))
-                          (pseudo-term-list-fix (cdr x)))
-                  nil)
-         :exec x)
-    ///
-    (more-returns
-     (new-x (<= (acl2-count new-x) (acl2-count x))
-            :name acl2-count-<=-pseudo-term-list-fix
-            :rule-classes :linear
-            :hints (("Goal" :in-theory (enable pseudo-term-fix))))
-     (new-x (implies (pseudo-term-listp x)
-                     (equal new-x x))
-            :name equal-pseudo-term-list-fix)
-     (new-x (implies (pseudo-term-listp x)
-                     (equal (len new-x) (len x)))
-            :name len-equal-pseudo-term-list-fix
-            :rule-classes :linear)))
-
-  (defthm pseudo-term-list-fix-idempotent-lemma
-    (equal (pseudo-term-list-fix (pseudo-term-list-fix x))
-           (pseudo-term-list-fix x))
-    :hints (("Goal" :in-theory (enable pseudo-term-list-fix))))
-
-  (deffixtype pseudo-term-list
-    :fix pseudo-term-list-fix
-    :pred pseudo-term-listp
-    :equiv pseudo-term-list-equiv
-    :define t)
-
-  (defthmd pseudo-term-listp-of-cdr-pseudo-termp
-    (implies (and (pseudo-termp term)
-                  (consp term)
-                  (not (equal (car term) 'quote)))
-             (pseudo-term-listp (cdr term)))
-    :hints (("Goal" :in-theory (enable pseudo-termp))))
-
-  (defthmd pseudo-termp-of-car-of-pseudo-term-listp
-    (implies (and (pseudo-term-listp term)
-                  (consp term))
-             (pseudo-termp (car term))))
-
-  (define pseudo-term-list-list-fix ((x pseudo-term-list-listp))
-    :returns (fixed pseudo-term-list-listp)
-    (mbe :logic (if (consp x)
-                    (cons (pseudo-term-list-fix (car x))
-                          (pseudo-term-list-list-fix (cdr x)))
-                  nil)
-         :exec x))
-
-  (defthm pseudo-term-list-list-fix-idempotent-lemma
-    (equal (pseudo-term-list-list-fix (pseudo-term-list-list-fix x))
-           (pseudo-term-list-list-fix x))
-    :hints (("Goal" :in-theory (enable pseudo-term-list-list-fix))))
-
-  (deffixtype pseudo-term-list-list
-    :fix pseudo-term-list-list-fix
-    :pred pseudo-term-list-listp
-    :equiv pseudo-term-list-list-equiv
-    :define t
-    :forward t
-    :topic pseudo-term-list-listp)
-
-  (defalist pseudo-term-alist
-    :key-type pseudo-term
-    :val-type pseudo-term
-    :pred pseudo-term-alistp
-    :true-listp t)
-
-  (define true-list-fix ((lst true-listp))
-    :parents (SMT-hint-interface)
-    :short "Fixing function for true-listp."
-    :returns (fixed-lst true-listp)
-    (mbe :logic (if (consp lst)
-                    (cons (car lst)
-                          (true-list-fix (cdr lst)))
-                  nil)
-         :exec lst))
-
-  (defthm true-list-fix-idempotent-lemma
-    (equal (true-list-fix (true-list-fix x))
-           (true-list-fix x))
-    :hints (("Goal" :in-theory (enable true-list-fix))))
-
-  (defthm true-list-fix-preserve-length
-    (equal (len (true-list-fix x))
-           (len x))
-    :hints (("Goal" :in-theory (enable true-list-fix))))
-
-  (deffixtype true-list
-    :fix true-list-fix
-    :pred true-listp
-    :equiv true-list-equiv
-    :define t
-    :forward t
-    :topic true-listp)
-
-  (local (in-theory (enable true-listp true-list-fix pseudo-termp
-                            pseudo-term-fix pseudo-term-listp pseudo-term-list-fix)))
-  ;; (define list-fix (x)
-  ;;   (declare (xargs :guard (listp x)))
-  ;;   :enabled t
-  ;;   (mbe :logic (if (listp x) x nil)
-  ;;        :exec x))
-
-  ;; (deffixtype list
-  ;;   :fix list-fix
-  ;;   :pred listp
-  ;;   :equiv list-equiv
-  ;;   :define t)
-
   (defprod hint-pair
     :parents (smtlink-hint)
-    ((thm pseudo-termp :default nil)       ;; a theorem statement about the variable
-     (hints true-listp :default nil)     ;; the hint for proving this theorem
-     )
-    :verbosep t)
+    ((thm pseudo-termp "A theorem statement"
+          :default nil)
+     (hints true-listp "The ACL2 hint for proving this theorem"
+            :default nil)
+     (name symbolp "The name of the theorem if already proven in ACL2"
+           :default nil)))
 
   (deflist hint-pair-list
     :parents (hint-pair)
     :elt-type hint-pair
-    :pred hint-pair-listp
     :true-listp t)
 
-  (define decl->type-reqfix ((x hint-pair-p))
-    :returns (fixed hint-pair-p)
-    (b* ((x (hint-pair-fix x))
-         (thm (hint-pair->thm x))
-         (hints (hint-pair->hints x)))
-      (make-hint-pair :thm (if (symbolp thm) thm nil)
-                      :hints (true-list-fix hints))))
-
-  (local (in-theory (enable decl->type-reqfix)))
   (defprod decl
     :parents (smtlink-hint)
     ((name symbolp :default nil)
-     (type hint-pair-p
-           :default (make-hint-pair)
-           :reqfix (decl->type-reqfix type))
-     (meta-extract-thms symbol-listp :default nil))
-    :require (symbolp (hint-pair->thm type)))
+     (type hint-pair-p :default (make-hint-pair))
+     ;; The fixer should be found in types;
+     ;; So we don't need fixer in function hints.
+     ;; (fixer symbolp :default nil)
+     ))
 
   (deflist decl-list
     :parents (decl)
     :elt-type decl
-    :pred decl-listp
     :true-listp t)
 
-  ;; (defalist decl-alist
-  ;;   :key-type symbol
-  ;;   :val-type decl
-  ;;   :pred decl-alistp)
-
-  ;; (define make-alist-decl-list ((decl-lst decl-listp))
-  ;;   :returns (decl-alist decl-alistp)
-  ;;   :measure (len decl-lst)
-  ;;   (b* ((decl-lst (decl-list-fix decl-lst))
-  ;;        ((unless (consp decl-lst)) nil)
-  ;;        ((cons first rest) decl-lst)
-  ;;        ((decl d) first))
-  ;;     (cons (cons d.name d) (make-alist-decl-list rest))))
-
-  (defprod func
+  (defprod smt-function
     :parents (smtlink-hint)
     ((name symbolp :default nil)
-     (formals decl-listp :default nil)
-     (guard hint-pair-p :default (make-hint-pair))
-     (returns decl-listp :default nil)            ;; belong to auxiliary hypotheses
-     (more-returns hint-pair-listp :default nil)  ;; belong to auxiliary hypotheses
      (expansion-depth natp :default 1)
-     (flattened-formals symbol-listp :default nil)
-     (flattened-returns symbol-listp :default nil)
-     (meta-extract-thms symbol-listp :default nil)))
+     (formals decl-list-p :default nil)
+     (returns decl-list-p :default nil)
+     ;; I'm not sure what's good of having guard,
+     ;; currently the hint is generated but is not used in Smtlink.
+     (guard hint-pair-p :default (make-hint-pair))
+     (more-returns hint-pair-list-p :default nil)))
 
-  (deflist func-list
-    :parents (func)
-    :elt-type func
-    :pred func-listp
+  (defoption maybe-smt-function smt-function-p)
+
+  (deflist smt-function-list
+    :parents (smt-function)
+    :elt-type smt-function-p
     :true-listp t)
 
-  (defalist func-alist
-    :key-type symbol
-    :val-type func
-    :true-listp t
-    :pred func-alistp)
+  (defprod prod
+    ((kind symbolp :default nil)
+     (constructor smt-function-p :default (make-smt-function))
+     (field-accessors smt-function-list-p :default nil)
+     (theorems hint-pair-list-p :default nil)))
 
-  (defthm func-p-of-assoc-equal-of-func-alist
-    (implies (and (func-alistp x)
-                  (symbolp y)
-                  (assoc-equal y x))
-             (and (consp (assoc-equal y x))
-                  (func-p (cdr (assoc-equal y x))))))
-
-  (defprod binding
-    :parents (smtlink-hint)
-    ((var symbolp :default nil)
-     (expr pseudo-termp :default nil)
-     (type symbolp :default nil)))
-
-  (deflist binding-list
-    :parents (binding)
-    :elt-type binding
-    :pred binding-listp
+  (deflist prod-list
+    :elt-type prod-p
     :true-listp t)
 
-  (defprod let-binding
-    :parents (smtlink-hint)
-    ((bindings binding-listp :default nil)
-     (hypotheses hint-pair-listp :default nil)))
+  (defprod option
+    ((some-prod prod-p :default (make-prod))
+     (none-prod prod-p :default (make-prod))))
 
-  ;; The hint structure that contain all hints for the verified clause
-  ;; processor.
-  ;;
-  ;; Fields:
-  ;; User fields:
-  ;; 1. functions: function definitions.
-  ;; 2. hypotheses: hypotheses to the G theorem.
-  ;; 3. main-hint: hints to the G' -> G theorem.
-  ;; 4. let-binding: binds expressions to variables, generalization.
-  ;; 5. fty: a list of fty types used in the theorem. Will be treated as
-  ;; algebraic datatypes in SMT solver.
-  ;; 6. int-to-rat: converts all integers to rationals.
-  ;; 7. smt-dir: where to put the generated python files. Default /tmp/z3_files
-  ;; 8. rm-file: configuration for whether to remove generated files.
-  ;; 9. smt-fname: configure the name of generated SMT theorem file.
-  ;; 10. smt-params: hints for parameter tuning of the SMT solver.
-  ;;
-  ;; Internal fields:
-  ;; 11. fty-info: an alist from fty functions to fty-info-p
-  ;; 12. fty-types: contains all fty type definitions for translation
-  ;; 13. fast-functions: internal field for storing a fast version of function
-  ;; definitions. Might be able to make the functions field a fast one after
-  ;; changing the user interface.
-  ;; 14. aux-hint-list: internal field for making a list of auxiliary hints.
-  ;; 15. type-decl-list: internal field for making a list of auxiliary type
-  ;; hints.
-  ;; 16. expanded-clause-w/-hint: internal field for storing the SMT theorem.
-  ;; 17. expanded-G/type: clause without type
-  ;; 18. smt-cnf: configuration for connection to the SMT solver.
-  ;; 19. wrld-fn-len: a number specifying the upper bound of the length of the
-  ;; current world. It sets a limit to the expansion depth to take care of
-  ;; recursive function expansion. This will only ensure termination proof of
-  ;; the expand function, but it doesn't guarantee performance since the world
-  ;; length can be extremely large, and expansion is exponential. Performance
-  ;; is replied upon user who will specify which functions are recursive and
-  ;; therefore will be expanded only by a given number of levels.
-  ;; 20. custom-p: Used custom version of Smtlink or not. Default nil.
-  ;;
-  (defprod smtlink-hint
-    :parents (SMT-hint-interface)
-    ((functions func-listp :default nil)
-     (hypotheses hint-pair-listp :default nil)
-     (main-hint true-listp :default nil)
-     (let-binding let-binding-p :default (make-let-binding))
-     (symbols symbol-listp :default nil)
-     (fty symbol-listp :default nil)
-     (fty-info fty-info-alist-p :default nil)
-     (fty-types fty-types-p :default nil)
-     (int-to-rat booleanp :default nil)
-     (smt-dir stringp :default "")
-     (rm-file booleanp :default t)
-     (smt-fname stringp :default "")
-     (smt-params true-listp :default nil)
-     (fast-functions func-alistp :default nil)
-     (type-decl-list pseudo-termp :default nil)
-     (expanded-clause-w/-hint hint-pair-p :default (make-hint-pair))
-     (expanded-G/type pseudo-termp :default nil)
-     (smt-cnf smtlink-config-p :default (make-smtlink-config))
-     (wrld-fn-len natp :default 0)
-     (custom-p booleanp :default nil)))
-
-  (defoption maybe-smtlink-hint smtlink-hint-p
-    :parents (smtlink-hint))
-
-  (define flatten-formals/returns ((formal/return-lst decl-listp))
-    :returns (mv (flattened-lst symbol-listp)
-                 (meta-extract-thms symbol-listp))
-    :measure (len formal/return-lst)
-    :hints (("Goal" :in-theory (enable decl-list-fix)))
-    (b* ((formal/return-lst (decl-list-fix formal/return-lst))
-         ((if (endp formal/return-lst)) (mv nil nil))
-         ((cons first rest) formal/return-lst)
-         ((decl d) first)
-         ((mv rest-formals/returns rest-meta)
-          (flatten-formals/returns rest)))
-      (mv (cons d.name rest-formals/returns)
-          (append d.meta-extract-thms rest-meta))))
-
-  (define make-alist-fn-lst ((fn-lst func-listp))
-    :parents (SMT-hint-interface)
-    :short "@(call make-alist-fn-lst) makes fn-lst a simpler alist"
-    :returns (fast-fn-lst func-alistp)
-    :measure (len fn-lst)
-    (b* ((fn-lst (func-list-fix fn-lst))
-         ((unless (consp fn-lst)) nil)
-         ((cons first rest) fn-lst)
-         ((func f) first)
-         ((mv formals &) (flatten-formals/returns f.formals))
-         ((mv returns meta) (flatten-formals/returns f.returns))
-         (new-f (change-func f
-                             :flattened-formals formals
-                             :flattened-returns returns
-                             :meta-extract-thms meta)))
-      (cons (cons f.name new-f) (make-alist-fn-lst rest))))
-
-  (define generate-fty-info-alist ((hints smtlink-hint-p)
-                                   (flextypes-table alistp))
-    :returns (updated-hints smtlink-hint-p)
-    (b* ((hints (smtlink-hint-fix hints))
-         ((smtlink-hint h) hints)
-         ((unless (alistp flextypes-table)) h)
-         (fty-info (generate-fty-info-alist-rec h.fty nil flextypes-table)))
-      (change-smtlink-hint h :fty-info fty-info)))
-
-  (local
-   (defthm crock-for-generate-fty-types-top
-     (implies (fty-types-p x)
-              (fty-types-p (reverse x)))))
-
-  (define generate-fty-types-top ((hints smtlink-hint-p)
-                                  (flextypes-table alistp))
-    :returns (updated-hints smtlink-hint-p)
-    (b* ((hints (smtlink-hint-fix hints))
-         ((smtlink-hint h) hints)
-         ((unless (alistp flextypes-table)) h)
-         ((mv & ordered-acc)
-          (generate-fty-type-list h.fty flextypes-table
-                                  h.fty-info nil nil))
-         (fty-types (reverse ordered-acc)))
-      (change-smtlink-hint h :fty-types fty-types)))
-
-  (defconst *default-smtlink-hint*
-    (make-smtlink-hint))
-
-
-  ;; (defstub smt-hint () => *)
-  (encapsulate
-    (((smt-hint) => *))
-    (local (define smt-hint () (make-smtlink-hint)))
-    (defthm smtlink-p-of-smt-hint
-      (smtlink-hint-p (smt-hint)))
+  (deftagsum smt-type
+    (:default ((constructor smt-function-p :default (make-smt-function))
+               (destructors smt-function-list-p :default nil)
+               (theorems hint-pair-list-p :default nil)))
+    (:list ((cons smt-function-p :default (make-smt-function))
+            (car smt-function-p :default (make-smt-function))
+            (cdr smt-function-p :default (make-smt-function))
+            (elt-type decl-p :default (decl))
+            (theorems hint-pair-list-p :default nil)))
+    (:array ((store smt-function-p :default (make-smt-function))
+             (select smt-function-p :default (make-smt-function))
+             (key-type decl-p :default (make-decl))
+             (val-type decl-p :default (make-decl))
+             (theorems hint-pair-list-p :default nil)))
+    (:prod ((prod prod-p :default (make-prod))))
+    (:option ((option option-p :default (make-option))))
+    ;; A prod and an option are all sums,
+    ;; we use sum here to denote more general sums
+    (:sum ((prods prod-list-p :default nil)))
+    (:uninterpreted ((constructor smt-function-p :default (make-smt-function))
+                     (destructors smt-function-list-p :default nil)
+                     (theorems hint-pair-list-p :default nil)))
     )
 
-  (define default-smtlink-hint ()
-    (change-smtlink-hint *default-smtlink-hint*))
+  (defprod smt-fixtype
+    :parents (smtlink-hint)
+    ((name symbolp)
+     (recognizer symbolp)
+     (fixer symbolp)
+     (fixer-when-recognizer-thm symbolp)
+     (type smt-type-p)))
 
-  (defattach smt-hint default-smtlink-hint)
+  (defoption maybe-smt-fixtype smt-fixtype-p)
 
+  (deflist smt-fixtype-list
+    :parents (smt-fixtype)
+    :elt-type smt-fixtype-p
+    :true-listp t)
+
+  (defprod smt-config
+    ((smt-cnf smtlink-config-p :default (make-smtlink-config))
+     (rm-file booleanp :default t)
+     (smt-dir stringp :default "")
+     (smt-fname stringp :default "")))
+
+  (deftagsum int-to-rat
+    (:switch ((okp booleanp :default nil)))
+    (:symbol-list ((lst symbol-listp :default nil))))
+
+  (local (in-theory (disable symbol-listp)))
+
+  (defprod smtlink-hint
+    :parents (SMT-hint-interface)
+    ((functions smt-function-list-p :default nil)
+     (types smt-fixtype-list-p :default nil)
+     (hypotheses hint-pair-list-p :default nil)
+     (configurations smt-config-p :default (make-smt-config))
+
+     (int-to-rat int-to-rat-p :default (make-int-to-rat-switch :okp nil))
+     (use-uninterpreted booleanp :default t)
+     (under-induct symbolp :default nil)
+     (global-hint symbolp :default nil)
+     (wrld-fn-len natp :default 0)
+     (custom-p booleanp :default nil)
+     ))
+
+  (defalist smtlink-hint-alist
+    :key-type symbolp
+    :val-type smtlink-hint-p
+    :true-listp t)
+
+  (defthm assoc-equal-of-smtlink-hint-alist
+    (implies (and (smtlink-hint-alist-p x)
+                  (consp (assoc-equal name x)))
+             (smtlink-hint-p (cdr (assoc-equal name x)))))
+  ;; ---------------------------------------------------------------
+  ;; Utility functions
+
+  ;; decl-list functions
+  (define get-thm-from-decl ((decl decl-p))
+    :returns (thm pseudo-termp)
+    (hint-pair->thm (decl->type (decl-fix decl))))
+
+  (define get-thms-from-decl-list ((dlst decl-list-p))
+    :returns (thms pseudo-term-listp)
+    :measure (len dlst)
+    (b* ((dlst (decl-list-fix dlst))
+         ((unless (consp dlst)) nil)
+         ((cons first rest) dlst))
+      (cons (get-thm-from-decl first)
+            (get-thms-from-decl-list rest))))
+
+  ;; smt-function-list functions
+  (define is-function ((name symbolp) (fn-lst smt-function-list-p))
+    :returns (f maybe-smt-function-p)
+    :measure (len fn-lst)
+    (b* ((fn-lst (smt-function-list-fix fn-lst))
+         ((unless (consp fn-lst)) nil)
+         ((cons first rest) fn-lst)
+         (first-name (smt-function->name first))
+         ((if (equal first-name name)) first))
+      (is-function name rest)))
+
+  ;; smt-fixtype-list functions
+  (define is-type ((x symbolp) (fixtypes smt-fixtype-list-p))
+    :returns (type maybe-smt-fixtype-p)
+    :measure (len fixtypes)
+    (b* ((fixtypes (smt-fixtype-list-fix fixtypes))
+         ((unless (consp fixtypes)) nil)
+         ((cons first rest) fixtypes)
+         ((if (equal x (smt-fixtype->recognizer first))) first))
+      (is-type x rest)))
+
+  (define is-recognizer ((x symbolp) (fixtypes smt-fixtype-list-p))
+    :returns (okp booleanp)
+    :measure (len fixtypes)
+    (b* ((fixtypes (smt-fixtype-list-fix fixtypes))
+         ((unless (consp fixtypes)) nil)
+         ((cons first rest) fixtypes)
+         ((if (equal x (smt-fixtype->recognizer first))) t))
+      (is-recognizer x rest)))
+
+  (define is-fixer ((x symbolp) (fixtypes smt-fixtype-list-p))
+    :returns (okp booleanp)
+    :measure (len fixtypes)
+    (b* ((fixtypes (smt-fixtype-list-fix fixtypes))
+         ((unless (consp fixtypes)) nil)
+         ((cons first rest) fixtypes)
+         ((if (equal x (smt-fixtype->fixer first))) t))
+      (is-fixer x rest)))
+
+  (define name-of-recognizer ((x symbolp) (fixtypes smt-fixtype-list-p))
+    :returns (name symbolp)
+    :measure (len fixtypes)
+    (b* ((fixtypes (smt-fixtype-list-fix fixtypes))
+         ((unless (consp fixtypes)) nil)
+         ((cons first rest) fixtypes)
+         ((if (equal x (smt-fixtype->recognizer first)))
+          (smt-fixtype->name first)))
+      (name-of-recognizer x rest)))
+
+  (define fncall-of-fixtypes ((x symbolp) (fixtypes smt-fixtype-list-p))
+    :returns (ok booleanp)
+    :ignore-ok t
+    nil)
+
+  (define fixer-of-recognizer ((x symbolp) (fixtypes smt-fixtype-list-p))
+    :returns (fixer symbolp)
+    :measure (len fixtypes)
+    (b* ((fixtypes (smt-fixtype-list-fix fixtypes))
+         ((unless (consp fixtypes)) nil)
+         ((cons first rest) fixtypes)
+         ((if (equal x (smt-fixtype->recognizer first)))
+          (smt-fixtype->fixer first)))
+      (fixer-of-recognizer x rest)))
+
+  (define recognizer-of-fixer ((x symbolp) (fixtypes smt-fixtype-list-p))
+    :returns (recognizer symbolp)
+    :measure (len fixtypes)
+    (b* ((fixtypes (smt-fixtype-list-fix fixtypes))
+         ((unless (consp fixtypes)) nil)
+         ((cons first rest) fixtypes)
+         ((if (equal x (smt-fixtype->fixer first)))
+          (smt-fixtype->recognizer first)))
+      (recognizer-of-fixer x rest)))
+
+  (define type-decl-p ((expr pseudo-termp)
+                       (fixtypes smt-fixtype-list-p))
+    :returns (is-decl? booleanp)
+    (b* (;; ((if (is-type-hyp-decl expr)) t)
+         ((unless (equal (len expr) 2))
+          nil)
+         (fn-name (car expr))
+         ((unless (symbolp fn-name)) nil)
+         ((unless (is-recognizer fn-name fixtypes))
+          nil)
+         ((unless (and (symbolp (cadr expr)) (cadr expr))) nil))
+      t)
+    ///
+    (more-returns
+     (is-decl?
+      (implies is-decl?
+               (and (consp expr)
+                    (consp (cdr expr))
+                    (symbolp (car expr))
+                    (is-recognizer (car expr) fixtypes)
+                    (symbolp (cadr expr)) (cadr expr)))
+      :name type-decl-p-definition)))
   )
+
+;; Put a default-hint into smt-hint-table
+(table smt-hint-table)
+
+(define get-smt-hint-table ((world plist-worldp))
+  (table-alist 'smt-hint-table world))
+
+(defmacro add-smtlink-hint (name hint)
+  (declare (xargs :guard (symbolp name)))
+  `(table smt-hint-table ',name ,hint))
+
+(add-smtlink-hint :default
+                  (make-smtlink-hint
+                   :configurations
+                   (make-smt-config :smt-cnf (default-smt-cnf))))
